Move aux tapes machine to its own file.

Cslib/Computability/Machines/MultiTapeTuring/AddRoutine.lean
@@ -20,91 +20,12 @@ public import Cslib.Computability.Machines.MultiTapeTuring.SequentialCombinator
 public import Cslib.Computability.Machines.MultiTapeTuring.WithTapes
 public import Cslib.Computability.Machines.MultiTapeTuring.IteCombinator
 public import Cslib.Computability.Machines.MultiTapeTuring.EqualRoutine
+public import Cslib.Computability.Machines.MultiTapeTuring.TMWithAuxTapes
 
 namespace Turing
 
 variable [Inhabited α] [Fintype α]
 variable {aux k : ℕ}
-
-public structure MultiTapeTMWithAuxTapes (k aux : ℕ) (α : Type)
-    extends MultiTapeTM (k + aux) α
-
---- We define `eval_list` only on the non-aux tapes and require that all aux tapes
---- start empty and have to be empty at the end of the computation.
-public noncomputable def MultiTapeTMWithAuxTapes.eval_list
-    (tm : MultiTapeTMWithAuxTapes k aux (WithSep α))
-    (tapes : Fin k → List (List α)) :
-    Part (Fin k → List (List α)) :=
-  ⟨∃ final_tapes, ∀ existing_tapes : Fin (k + aux) → List (List α),
-    tm.TransformsLists
-      -- TODO maybe we need "extends" and "restrictns" functions for tapes.
-      (fun i => if h : i < k then tapes ⟨i, h⟩ else existing_tapes ⟨i, by omega⟩)
-      (fun i => if h : i < k then final_tapes ⟨i, h⟩ else existing_tapes ⟨i, by omega⟩),
-    fun h => h.choose⟩
-
---- Require a minimum number of auxiliary tapes, adding new ones if needed.
-public def MultiTapeTMWithAuxTapes.require_aux_tapes
-  (tm : MultiTapeTMWithAuxTapes k aux α) (aux' : ℕ) :
-    MultiTapeTMWithAuxTapes k (max aux aux') α where
-  toMultiTapeTM := tm.toMultiTapeTM.extend (by omega)
-
---- Adds an additional number auf auxiliary tapes.
-public def MultiTapeTMWithAuxTapes.add_aux_tapes (tm : MultiTapeTMWithAuxTapes k aux α) (aux' : ℕ) :
-    MultiTapeTMWithAuxTapes k (aux + aux') α where
-  toMultiTapeTM := tm.toMultiTapeTM.extend (by omega)
-
---- Adds `aux` many tapes to the TM, which are guaranteed to be restored to their original
---- content at the end of the computation.
-public def MultiTapeTM.allocate_aux_tapes (tm : MultiTapeTM k α) (aux : ℕ) :
-    MultiTapeTMWithAuxTapes k aux α where
-  toMultiTapeTM := tm.extend (by omega)
-
-instance : Coe (MultiTapeTM k α) (MultiTapeTMWithAuxTapes k 0 α) where
-  coe tm := tm.allocate_aux_tapes 0
-
---- Sets the last `aux` many tapes to be aux tapes, which are guaranteed to be restored to their
---- original content at the end of the computation.
-@[simp, grind =]
-public def MultiTapeTM.set_aux_tapes (aux : ℕ) (tm : MultiTapeTM (k + aux) α) :
-    MultiTapeTMWithAuxTapes k aux α where
-  toMultiTapeTM := tm
-
---- Turn a TM with `k₁` tapes and `aux₁` many aux tapes into a TM with `k₂` tapes and `aux₂` many
---- aux tapes, where `seq` specifies which tapes of the new TM correspond to the tapes of the
---- old TM. Aux tapes are just assigned in order.
-public def MultiTapeTMWithAuxTapes.with_tapes
-  {aux₁ aux₂ k₁ k₂ : ℕ}
-  {h_le_k : k₁ ≤ k₂}
-  {h_le_aux : aux₁ ≤ aux₂}
-  (tm : MultiTapeTMWithAuxTapes k₁ aux₁ α)
-  (seq : Vector (Fin k₂) k₁) : MultiTapeTMWithAuxTapes k₂ aux₂ α :=
-  (tm.toMultiTapeTM.with_tapes (h_le := by omega) (
-    ((seq.map fun (t : Fin k₂) => (⟨t, by omega⟩)) : (Vector (Fin (k₂ + aux₂)) k₁)) ++
-    (((.ofFn fun i => ⟨k₂ + i, by omega⟩) : (Vector (Fin (k₂ + aux₂)) aux₁))))).set_aux_tapes aux₂
-
---- Run tm₂ after tm₁ has terminated.
-public def MultiTapeTMWithAuxTapes.seq (tm₁ tm₂ : MultiTapeTMWithAuxTapes k aux α) : MultiTapeTMWithAuxTapes k aux α :=
-  sorry
-
--- TODO this requires the auxiliary tapes to be empty between the two computations (because of
--- the use of MultiTapeTMWithAuxTapes.eval_list).
--- Do we need that?
-@[simp, grind=]
-public theorem MultiTapeTMWithAuxTapes.seq_eval_list
-  {tm₁ tm₂ : MultiTapeTMWithAuxTapes k aux (WithSep α)}
-  {tapes₀ : Fin k → List (List α)} :
-  (seq tm₁ tm₂).eval_list tapes₀ =
-    tm₁.eval_list tapes₀ >>= fun tape₁ => tm₂.eval_list tape₁ := by
-  sorry
-
-public theorem MultiTapeTMWithAuxTapes.seq_associative
-  (tm₁ tm₂ tm₃ : MultiTapeTMWithAuxTapes k aux α)
-  (tapes₀ : Fin k → List (List α)) :
-  (seq (seq tm₁ tm₂) tm₃).eval = (seq tm₁ (seq tm₂ tm₃)).eval := by
-  sorry
-
-infixl:90 " <;a> " => MultiTapeTMWithAuxTapes.seq
-
 
 namespace Routines
 
