Cslib/Computability/Machines/MultiTapeTuring/TMWithAuxTapes.lean
@@ -1,0 +1,113 @@
+/-
+Copyright (c) 2026 Christian Reitwiessner. All rights reserved.
+Released under Apache 2.0 license as described in the file LICENSE.
+Authors: Christian Reitwiessner
+-/
+
+module
+
+import Cslib.Foundations.Data.BiTape
+import Cslib.Foundations.Data.RelatesInSteps
+
+public import Cslib.Computability.Machines.MultiTapeTuring.Basic
+public import Cslib.Computability.Machines.MultiTapeTuring.ListEncoding
+public import Cslib.Computability.Machines.MultiTapeTuring.SuccRoutine
+public import Cslib.Computability.Machines.MultiTapeTuring.CopyRoutine
+public import Cslib.Computability.Machines.MultiTapeTuring.PushRoutine
+public import Cslib.Computability.Machines.MultiTapeTuring.PopRoutine
+public import Cslib.Computability.Machines.MultiTapeTuring.WhileCombinator
+public import Cslib.Computability.Machines.MultiTapeTuring.SequentialCombinator
+public import Cslib.Computability.Machines.MultiTapeTuring.WithTapes
+public import Cslib.Computability.Machines.MultiTapeTuring.IteCombinator
+public import Cslib.Computability.Machines.MultiTapeTuring.EqualRoutine
+
+namespace Turing
+
+variable [Inhabited α] [Fintype α]
+variable {aux k : ℕ}
+
+--- A Turing machine with a set of auxiliary tapes that are the last of the general tapes.
+--- The auxiliary tapes are only relevant for the semantics of the machine:
+--- The machine is required to reset the contents and head position of the auxiliary
+--- tapes to their original values at the end of the computation.
+public structure MultiTapeTMWithAuxTapes (k aux : ℕ) (α : Type)
+    extends MultiTapeTM (k + aux) α
+
+--- Adds `aux` many tapes to the TM, which are guaranteed to be restored to their original
+--- content at the end of the computation.
+@[simp, grind =]
+public def MultiTapeTM.allocate_aux_tapes (tm : MultiTapeTM k α) (aux : ℕ) :
+    MultiTapeTMWithAuxTapes k aux α where
+  toMultiTapeTM := tm.extend (by omega)
+
+--- Sets the last `aux` many tapes to be aux tapes, which are guaranteed to be restored to their
+--- original content at the end of the computation.
+@[simp, grind =]
+public def MultiTapeTM.set_aux_tapes (aux : ℕ) (tm : MultiTapeTM (k + aux) α) :
+    MultiTapeTMWithAuxTapes k aux α where
+  toMultiTapeTM := tm
+
+instance : Coe (MultiTapeTM k α) (MultiTapeTMWithAuxTapes k 0 α) where
+  coe tm := tm.allocate_aux_tapes 0
+
+namespace MultiTapeTMWithAuxTapes
+
+--- We define `eval_list` only on the non-aux tapes and require that all aux tapes
+--- are reset to their original contents.
+public noncomputable def eval_list
+    (tm : MultiTapeTMWithAuxTapes k aux (WithSep α))
+    (tapes : Fin k → List (List α)) :
+    Part (Fin k → List (List α)) :=
+  ⟨∃ final_tapes, ∀ existing_tapes : Fin (k + aux) → List (List α),
+    tm.TransformsLists
+      -- TODO maybe we need "extends" and "restricts" functions for tapes.
+      (fun i => if h : i < k then tapes ⟨i, h⟩ else existing_tapes ⟨i, by omega⟩)
+      (fun i => if h : i < k then final_tapes ⟨i, h⟩ else existing_tapes ⟨i, by omega⟩),
+    fun h => h.choose⟩
+
+--- Require a minimum number of auxiliary tapes, adding new ones if needed.
+public def require_aux_tapes
+  (tm : MultiTapeTMWithAuxTapes k aux α) (aux' : ℕ) :
+    MultiTapeTMWithAuxTapes k (max aux aux') α where
+  toMultiTapeTM := tm.toMultiTapeTM.extend (by omega)
+
+
+--- Turn a TM with `k₁` tapes and `aux₁` many aux tapes into a TM with `k₂` tapes and `aux₂` many
+--- aux tapes, where `seq` specifies which tapes of the new TM correspond to the tapes of the
+--- old TM. Aux tapes are just assigned in order.
+public def with_tapes
+  {aux₁ aux₂ k₁ k₂ : ℕ}
+  {h_le_k : k₁ ≤ k₂}
+  {h_le_aux : aux₁ ≤ aux₂}
+  (tm : MultiTapeTMWithAuxTapes k₁ aux₁ α)
+  (seq : Vector (Fin k₂) k₁) : MultiTapeTMWithAuxTapes k₂ aux₂ α :=
+  (tm.toMultiTapeTM.with_tapes (h_le := by omega) (
+    ((seq.map fun (t : Fin k₂) => (⟨t, by omega⟩)) : (Vector (Fin (k₂ + aux₂)) k₁)) ++
+    (((.ofFn fun i => ⟨k₂ + i, by omega⟩) : (Vector (Fin (k₂ + aux₂)) aux₁))))).set_aux_tapes aux₂
+
+--- Run tm₂ after tm₁ has terminated.
+public def seq (tm₁ tm₂ : MultiTapeTMWithAuxTapes k aux α) : MultiTapeTMWithAuxTapes k aux α :=
+  sorry
+
+-- TODO this requires the auxiliary tapes to be empty between the two computations (because of
+-- the use of eval_list).
+-- Do we need that?
+@[simp, grind=]
+public theorem seq_eval_list
+  {tm₁ tm₂ : MultiTapeTMWithAuxTapes k aux (WithSep α)}
+  {tapes₀ : Fin k → List (List α)} :
+  (seq tm₁ tm₂).eval_list tapes₀ =
+    tm₁.eval_list tapes₀ >>= fun tape₁ => tm₂.eval_list tape₁ := by
+  sorry
+
+public theorem seq_associative
+  (tm₁ tm₂ tm₃ : MultiTapeTMWithAuxTapes k aux α)
+  (tapes₀ : Fin k → List (List α)) :
+  (seq (seq tm₁ tm₂) tm₃).eval = (seq tm₁ (seq tm₂ tm₃)).eval := by
+  sorry
+
+infixl:90 " <;a> " => seq
+
+end MultiTapeTMWithAuxTapes
+
+end Turing
